Iris/Iris/HeapLang/Lib/SpinLock.lean
@@ -8,14 +8,14 @@ public import Iris.HeapLang.PrimitiveLaws
 
 namespace Iris.HeapLang
 
-open BI Iris
+open BI Iris ProgramLogic
 
 @[expose] public section
 
 def spinlock_newlock : Val := hl_val(λ _, ref(#false))
-def spinlock_try_acquire : Val := hl_val(λ l, cas(l, #false, #true))
+def spinlock_try_acquire : Val := hl_val(λ l, snd(cmpXchg(l, #false, #true)))
 def spinlock_acquire : Val :=
-  hl_val(rec acquire l := if {spinlock_try_acquire} l then #() else acquire l)
+  hl_val(rec acquire l := if ({spinlock_try_acquire} l) then #() else acquire l)
 def spinlock_release : Val := hl_val(λ l, l ← #false)
 
 abbrev SpinLockG (GF : BundledGFunctors) := TokenG GF
@@ -29,7 +29,7 @@ variable [HeapLangGS hlc GF] [SpinLockG GF]
 def locked (γ : GName) : IProp GF := token γ
 
 def lock_inv (γ : GName) (l : Loc) (R : IProp GF) : IProp GF :=
-  iprop(∃ b : Bool, (l ↦ Option.some hl_val(#b)) ∗ (if b then True else token γ ∗ R))
+  iprop(∃ b : Bool, (l ↦ Option.some hl_val(#b)) ∗ (if b then True else locked γ ∗ R))
 
 def is_lock (γ : GName) (lk : Val) (R : IProp GF) : IProp GF :=
   iprop(∃ l : Loc, ⌜lk = Val.lit (.loc l)⌝ ∧ inv spinlockN (lock_inv γ l R))
@@ -95,30 +95,126 @@ theorem spinlock_newlock_spec :
     unfold is_lock
     iexists l
     isplit; itrivial
-    unfold lock_inv
+    unfold lock_inv locked
     iframe
 
 theorem spinlock_try_acquire_spec (γ : GName) (lk : Val) (R : IProp GF) :
     ⊢ □ ∀ (Φ : Val → IProp GF),
     is_lock γ lk R
-    -∗ (((locked γ ∗ R) -∗ Φ (.lit (.bool true))) ∧
-     (True -∗ Φ (.lit (.bool false))))
+    -∗ (∀ (b : Bool), iprop(if b then locked γ ∗ R else iprop(True)) -∗ Φ hl_val(#b))
     -∗ WP hl({spinlock_try_acquire} {lk}) {{ Φ }} := by
-  sorry
+  unfold spinlock_try_acquire
+  imodintro
+  iintro %Φ #Hlock Hcont
+  iapply wp_rec; simp only [Exp.subst, Exp.substStr, BEq.rfl, ↓reduceIte]
+  inext
+  unfold is_lock
+  icases Hlock with ⟨%l, %Heq, #Hinv⟩
+  subst Heq
+  iapply wp_bind (fun x => hl(snd({x})))
+  iapply wp_atomic (E2 := ⊤ \ nclose spinlockN)
+  imod inv_acc ⊤ _ _ (fun _ _ => CoPset.mem_full) $$ Hinv with ⟨G1, G2⟩
+  unfold lock_inv
+  imodintro
+  icases G1 with ⟨%b, Hpt, Hcond⟩
+  cases b
+  · simp only [Bool.false_eq_true, ↓reduceIte]
+    iapply wp_wand $$ [Hpt]
+    · iapply wp_cmpXchg_true (e1 := hl(#(BaseLit.bool false)))
+        (e2 := hl(#(BaseLit.bool true))) $$ Hpt
+      · simp [toVal]; rfl
+      · simp [toVal]; rfl
+      · simp [Val.compareSafe, Val.isUnboxed, BaseLit.isUnboxed]
+      · simp
+    iintro %v ⟨%Heq, Hpt⟩
+    subst Heq
+    imod G2 $$ [Hpt]
+    · iexists true
+      simp only [↓reduceIte]
+      iframe
+    · imodintro
+      iapply wp_snd
+      inext
+      iapply Hcont $$ [Hcond]
+      simp only [↓reduceIte]
+      iframe
+  · simp only [↓reduceIte]
+    iapply wp_wand $$ [Hpt]
+    · iapply wp_cmpXchg_fail (e1 := hl(#(BaseLit.bool false)))
+        (e2 := hl(#(BaseLit.bool true))) $$ Hpt
+      · simp [toVal]; rfl
+      · simp [toVal]; rfl
+      · simp [Val.compareSafe, Val.isUnboxed, BaseLit.isUnboxed]
+      · simp
+    iintro %v ⟨%Heq, Hpt⟩
+    subst Heq
+    imod G2 $$ [Hpt]
+    · iexists true
+      simp only [↓reduceIte]
+      iframe
+    · imodintro
+      iapply wp_snd
+      inext
+      iapply Hcont $$ [Hcond]
+      simp only [Bool.false_eq_true, ↓reduceIte]
+      itrivial
 
 theorem spinlock_acquire_spec (γ : GName) (lk : Val) (R : IProp GF) :
   ⊢ □ ∀ (Φ : Val → IProp GF),
     is_lock γ lk R
-    -∗ ((locked γ ∗ R) -∗ Φ (.lit .unit))
+    -∗ (locked γ ∗ R -∗ Φ hl_val(#()))
     -∗ WP hl({spinlock_acquire} {lk}) {{ Φ }} := by
-  sorry
+  unfold spinlock_acquire
+  iintro !> %Φ #Hlock Hcont
+  iloeb as IH
+  iapply wp_rec; simp only [Exp.subst, Exp.substStr, String.reduceBEq, Bool.false_eq_true,
+    ↓reduceIte, BEq.rfl]
+  inext
+  iapply wp_bind (fun x => hl(if {x} then {?_} else {?_})) (κ := instContextExpValStateObservationIf)
+  iapply spinlock_try_acquire_spec $$ Hlock
+  iintro %b Hpt
+  cases b
+  · iapply wp_if_false
+    inext
+    iapply IH
+    iapply Hcont
+  · iapply wp_if_true
+    inext
+    iapply wp_value'
+    iapply Hcont
+    simp only [if_pos]
+    iframe
 
 theorem spinlock_release_spec (γ : GName) (lk : Val) (R : IProp GF) :
   ⊢ □ ∀ (Φ : Val → IProp GF),
-    (is_lock γ lk R ∗ locked γ ∗ R)
-    -∗ (True -∗ Φ (.lit .unit))
+    is_lock γ lk R ∗ (locked γ ∗ R)
+    -∗ (True -∗ Φ hl_val(#()))
     -∗ WP hl({spinlock_release} {lk}) {{ Φ }} := by
-  sorry
+  unfold spinlock_release
+  iintro !> %Φ ⟨#Hlock, ⟨Hl, HR⟩⟩ Hcont
+  iapply wp_rec; simp only [Exp.subst, Exp.substStr, ↓reduceIte, BEq.rfl]
+  inext
+  unfold is_lock
+  icases Hlock with ⟨%l, %Heq, #Hinv⟩
+  subst Heq
+  iapply wp_atomic (E2 := ⊤ \ nclose spinlockN)
+  imod inv_acc ⊤ _ _ (fun _ _ => CoPset.mem_full) $$ Hinv with ⟨G1, G2⟩
+  unfold lock_inv
+  imodintro
+  icases G1 with ⟨%b, Hpt, Hcond⟩
+  iapply wp_wand $$ [Hpt]
+  · iapply wp_store (e := hl(#(BaseLit.bool false))) $$ Hpt
+    simp [toVal]
+  iintro %_ ⟨%Heq, Hpt'⟩
+  subst Heq
+  imod G2 $$ [- Hcont]
+  · inext
+    iexists false
+    simp only [Bool.false_eq_true, ↓reduceIte]
+    iframe Hpt'  Hl HR
+  · imodintro
+    iapply Hcont
+    itrivial
 
 end SpinLockSpecs
 
@@ -135,8 +231,8 @@ def spinLock [HeapLangGS hlc GF] : lock GF where
   is_lock_iff γ lk R₁ R₂ := is_lock_iff γ lk R₁ R₂
   locked_timeless γ := locked_timeless γ
   locked_exclusive γ := locked_exclusive γ
-  newlock_spec_delay_init Φ := spinlock_newlock_spec Φ
-  acquire_spec γ lk R Φ := spinlock_acquire_spec γ lk R Φ
-  release_spec γ lk R Φ := spinlock_release_spec γ lk R Φ
+  newlock_spec_delay_init := spinlock_newlock_spec
+  acquire_spec γ lk R := spinlock_acquire_spec γ lk R
+  release_spec γ lk R := spinlock_release_spec γ lk R
 
 end
